Rewriting.

theories/std/raw_array.v
@@ -26,6 +26,9 @@ Qed.
 
 Section raw_array_G.
   Context `{raw_array_G : RawArrayG Σ}.
+  Implicit Types sz i j : nat.
+  Implicit Types l : loc.
+  Implicit Types v t : val.
 
   Definition raw_array_make : val :=
     λ: "sz" "v",
@@ -38,13 +41,6 @@ Section raw_array_G.
     λ: "t" "i" "v",
       "t" +ₗ "i" <- "v".
 
-  #[local] Definition raw_array_name := gname.
-
-  Implicit Types sz i j : nat.
-  Implicit Types l : loc.
-  Implicit Types v t : val.
-  Implicit Types γ : raw_array_name.
-
   Section raw_array_token.
     #[local] Definition raw_array_token_auth γ sz :=
       auth_nat_max_auth γ DfracDiscarded sz.
@@ -55,8 +51,8 @@ Section raw_array_G.
       ⊢ |==> ∃ γ,
         raw_array_token_auth γ sz.
     Proof.
-      iMod auth_nat_max_alloc as "(%γ & H●)".
-      iMod (auth_nat_max_auth_persist with "H●") as "H●".
+      iMod auth_nat_max_alloc as "(%γ & Hauth)".
+      iMod (auth_nat_max_auth_persist with "Hauth") as "Hauth".
       iExists γ. done.
     Qed.
     #[local] Lemma raw_array_token_valid γ sz i :
@@ -64,22 +60,21 @@ Section raw_array_G.
       raw_array_token_lb γ i -∗
       ⌜i ≤ sz⌝.
     Proof.
-      iApply auth_nat_max_valid.
+      apply auth_nat_max_valid.
     Qed.
     #[local] Lemma raw_array_token_lb_le γ i i' :
       i' ≤ i →
       raw_array_token_lb γ i -∗
       raw_array_token_lb γ i'.
     Proof.
-      intros. iApply auth_nat_max_lb_le. done.
+      apply auth_nat_max_lb_le.
     Qed.
   End raw_array_token.
 
   Section raw_array_inv.
     Definition raw_array_inv t sz : iProp Σ :=
       ∃ l γ,
-      ⌜t = #l⌝ ∗
-      meta l nroot γ ∗
+      ⌜t = #l⌝ ∗ meta l nroot γ ∗
       ⌜0 < sz⌝ ∗ raw_array_token_auth γ sz.
 
     #[global] Instance raw_array_inv_persistent t sz :
@@ -92,15 +87,14 @@ Section raw_array_G.
       raw_array_inv t sz -∗
       ⌜0 < sz⌝.
     Proof.
-      iIntros "(%l & %γ & -> & #Hmeta & $ & #H●)".
+      iIntros "(%l & %γ & -> & #Hmeta & $ & #Hauth)".
     Qed.
   End raw_array_inv.
 
   Section raw_array_mapsto.
     Definition raw_array_mapsto t i dq v : iProp Σ :=
       ∃ l γ,
-      ⌜t = #l⌝ ∗
-      meta l nroot γ ∗
+      ⌜t = #l⌝ ∗ meta l nroot γ ∗
       raw_array_token_lb γ (S i) ∗
       (l +ₗ i) ↦{dq} v.
 
@@ -110,7 +104,7 @@ Section raw_array_G.
       apply _.
     Qed.
     #[global] Instance raw_array_mapsto_persistent t i v :
-      Timeless (raw_array_mapsto t i DfracDiscarded v).
+      Persistent (raw_array_mapsto t i DfracDiscarded v).
     Proof.
       apply _.
     Qed.
@@ -119,9 +113,9 @@ Section raw_array_G.
       Fractional (λ q, raw_array_mapsto t i (DfracOwn q) v).
     Proof.
       intros q1 q2. iSplit.
-      - iIntros "(%l & %γ & -> & #Hmeta & #H◯ & H↦1 & H↦2)".
+      - iIntros "(%l & %γ & -> & #Hmeta & #Hlb & H↦1 & H↦2)".
         iSplitL "H↦1"; repeat iExists _; naive_solver.
-      - iIntros "((%l1 & %γ1 & % & #Hmeta1 & #H◯ & H↦1) & (%l2 & %γ2 & % & #Hmeta2 & _ & H↦2))". simplify.
+      - iIntros "((%l1 & %γ1 & % & #Hmeta1 & #Hlb & H↦1) & (%l2 & %γ2 & % & #Hmeta2 & _ & H↦2))". simplify.
         iDestruct (meta_agree with "Hmeta1 Hmeta2") as %->.
         repeat iExists _. iFrame. naive_solver.
     Qed.
@@ -131,34 +125,61 @@ Section raw_array_G.
       split; [done | apply _].
     Qed.
 
-    Lemma raw_array_mapsto_persist t i dq v :
-      raw_array_mapsto t i dq v ==∗
-      raw_array_mapsto t i DfracDiscarded v.
-    Proof.
-      iIntros "(%l & %γ & -> & Hmeta & #H◯ & H↦)".
-      iMod (mapsto_persist with "H↦").
-      repeat iExists _. naive_solver.
-    Qed.
-
     Lemma raw_array_mapsto_valid t sz i dq v :
       raw_array_inv t sz -∗
       raw_array_mapsto t i dq v -∗
       ⌜✓ dq ∧ i < sz⌝.
     Proof.
-      iIntros "(%l & %γ & % & #Hmeta & % & #H●) (%_l & %_γ & -> & #_Hmeta & #H◯ & H↦)". simplify.
+      iIntros "(%l & %γ & % & #Hmeta & % & #Hauth) (%_l & %_γ & -> & #_Hmeta & #Hlb & H↦)". simplify.
       iDestruct (meta_agree with "Hmeta _Hmeta") as %<-. iClear "_Hmeta".
       iDestruct (mapsto_valid with "H↦") as %?.
-      iDestruct (raw_array_token_valid with "H● H◯") as %?. done.
+      iDestruct (raw_array_token_valid with "Hauth Hlb") as %?. done.
     Qed.
     Lemma raw_array_mapsto_valid_2 t i dq1 v1 dq2 v2 :
       raw_array_mapsto t i dq1 v1 -∗
       raw_array_mapsto t i dq2 v2 -∗
       ⌜✓ (dq1 ⋅ dq2) ∧ v1 = v2⌝.
     Proof.
-      iIntros "(%l1 & %γ1 & % & #Hmeta1 & #H◯1 & H↦1) (%l2 & %γ2 & % & #Hmeta2 & #H◯2 & H↦2)". simplify.
+      iIntros "(%l1 & %γ1 & % & #Hmeta1 & #Hlb1 & H↦1) (%l2 & %γ2 & % & #Hmeta2 & #Hlb2 & H↦2)". simplify.
       iDestruct (mapsto_valid_2 with "H↦1 H↦2") as %?. done.
     Qed.
-
+    Lemma raw_array_mapsto_combine t i dq1 v1 dq2 v2 :
+      raw_array_mapsto t i dq1 v1 -∗
+      raw_array_mapsto t i dq2 v2 -∗
+        raw_array_mapsto t i (dq1 ⋅ dq2) v1 ∗
+        ⌜v1 = v2⌝.
+    Proof.
+      iIntros "Hmapsto1 Hmapsto2".
+      iDestruct (raw_array_mapsto_valid_2 with "Hmapsto1 Hmapsto2") as %(_ & ->).
+      iDestruct "Hmapsto1" as "(%l & %γ & % & #Hmeta1 & #Hlb1 & H↦1)".
+      iDestruct "Hmapsto2" as "(%_l & %_γ & -> & #_Hmeta & #Hlb2 & H↦2)". simplify.
+      iDestruct (mapsto_combine with "H↦1 H↦2") as "(H↦ & _)".
+      iSplit; last done. repeat iExists _. naive_solver.
+    Qed.
+    Lemma raw_array_mapsto_agree t i dq1 v1 dq2 v2 :
+      raw_array_mapsto t i dq1 v1 -∗
+      raw_array_mapsto t i dq2 v2 -∗
+      ⌜v1 = v2⌝.
+    Proof.
+      iIntros "Hmapsto1 Hmapsto2".
+      iDestruct (raw_array_mapsto_combine with "Hmapsto1 Hmapsto2") as "(_ & ->)"; done.
+    Qed.
+    Lemma raw_array_mapsto_dfrac_ne i t1 dq1 v1 t2 dq2 v2 :
+      ¬ ✓ (dq1 ⋅ dq2) →
+      raw_array_mapsto t1 i dq1 v1 -∗
+      raw_array_mapsto t2 i dq2 v2 -∗
+      ⌜t1 ≠ t2⌝.
+    Proof.
+      iIntros "% Hmapsto1 Hmapsto2" (->).
+      iDestruct (raw_array_mapsto_valid_2 with "Hmapsto1 Hmapsto2") as %?; naive_solver.
+    Qed.
+    Lemma raw_array_mapsto_ne i t1 v1 t2 dq2 v2 :
+      raw_array_mapsto t1 i (DfracOwn 1) v1 -∗
+      raw_array_mapsto t2 i dq2 v2 -∗
+      ⌜t1 ≠ t2⌝.
+    Proof.
+      intros. iApply raw_array_mapsto_dfrac_ne; [done.. | intros []%(exclusive_l _)].
+    Qed.
     Lemma raw_array_mapsto_exclusive t i v1 v2 :
       raw_array_mapsto t i (DfracOwn 1) v1 -∗
       raw_array_mapsto t i (DfracOwn 1) v2 -∗
@@ -167,17 +188,12 @@ Section raw_array_G.
       iIntros "Hmapsto1 Hmapsto2".
       iDestruct (raw_array_mapsto_valid_2 with "Hmapsto1 Hmapsto2") as %(?%dfrac_valid_own_r & _). done.
     Qed.
-
-    Lemma raw_array_mapsto_combine t i dq1 v1 dq2 v2 :
-      raw_array_mapsto t i dq1 v1 -∗
-      raw_array_mapsto t i dq2 v2 -∗
-      raw_array_mapsto t i (dq1 ⋅ dq2) v1.
+    Lemma raw_array_mapsto_persist t i dq v :
+      raw_array_mapsto t i dq v ==∗
+      raw_array_mapsto t i DfracDiscarded v.
     Proof.
-      iIntros "Hmapsto1 Hmapsto2".
-      iDestruct (raw_array_mapsto_valid_2 with "Hmapsto1 Hmapsto2") as %(_ & ->).
-      iDestruct "Hmapsto1" as "(%l & %γ & % & #Hmeta1 & #H◯1 & H↦1)".
-      iDestruct "Hmapsto2" as "(%_l & %_γ & -> & #_Hmeta & #H◯2 & H↦2)". simplify.
-      iDestruct (mapsto_combine with "H↦1 H↦2") as "(H↦ & _)".
+      iIntros "(%l & %γ & -> & Hmeta & #Hlb & H↦)".
+      iMod (mapsto_persist with "H↦").
       repeat iExists _. naive_solver.
     Qed.
   End raw_array_mapsto.
@@ -185,8 +201,7 @@ Section raw_array_G.
   Section raw_array_view.
     Definition raw_array_view t i dq vs : iProp Σ :=
       ∃ l γ,
-      ⌜t = #l⌝ ∗
-      meta l nroot γ ∗
+      ⌜t = #l⌝ ∗ meta l nroot γ ∗
       raw_array_token_lb γ (i + length vs) ∗
       [∗ list] j ↦ v ∈ vs, (l +ₗ (i + j)%nat) ↦{dq} v.
 
@@ -196,7 +211,7 @@ Section raw_array_G.
       apply _.
     Qed.
     #[global] Instance raw_array_view_persistent t i vs :
-      Timeless (raw_array_view t i DfracDiscarded vs).
+      Persistent (raw_array_view t i DfracDiscarded vs).
     Proof.
       apply _.
     Qed.
@@ -205,10 +220,10 @@ Section raw_array_G.
       Fractional (λ q, raw_array_view t i (DfracOwn q) vs).
     Proof.
       intros q1 q2. iSplit.
-      - iIntros "(%l & %γ & % & #Hmeta & #H◯ & Hvs)". simplify.
+      - iIntros "(%l & %γ & % & #Hmeta & #Hlb & Hvs)". simplify.
         iDestruct (fractional_big_sepL vs (λ j v q, (l +ₗ (i + j)%nat) ↦{#q} v)%I with "Hvs") as "(Hvs1 & Hvs2)".
         iSplitL "Hvs1"; repeat iExists _; naive_solver.
-      - iIntros "((%l1 & %γ1 & % & #Hmeta1 & #H◯1 & Hvs1) & (%l2 & %γ2 & % & #Hmeta2 & #H◯2 & Hvs2))". simplify.
+      - iIntros "((%l1 & %γ1 & % & #Hmeta1 & #Hlb1 & Hvs1) & (%l2 & %γ2 & % & #Hmeta2 & #Hlb2 & Hvs2))". simplify.
         iDestruct (meta_agree with "Hmeta1 Hmeta2") as %->.
         iDestruct (fractional_big_sepL vs (λ j v q, (l2 +ₗ (i + j)%nat) ↦{#q} v)%I with "[$Hvs1 $Hvs2]") as "Hvs".
         repeat iExists _; naive_solver.
@@ -226,11 +241,11 @@ Section raw_array_G.
         raw_array_token_lb γ (i + length vs) ∗
         [∗ list] j ↦ v ∈ vs, raw_array_mapsto t (i + j) dq v.
     Proof.
-      iIntros "(%l & %γ & -> & #Hmeta & #H◯ & H↦s)".
+      iIntros "(%l & %γ & -> & #Hmeta & #Hlb & H↦s)".
       iExists l, γ. iFrame "∗#". iSplit; first done.
       iApply (big_sepL_impl with "H↦s"). iIntros "!> %j %v %Hlookup H↦".
       iExists l, γ. repeat iSplit; try done.
-      iApply (raw_array_token_lb_le with "H◯").
+      iApply (raw_array_token_lb_le with "Hlb").
       apply lookup_lt_Some in Hlookup. lia.
     Qed.
     Lemma raw_array_view_to_mapstos t i dq vs :
@@ -250,7 +265,7 @@ Section raw_array_G.
         raw_array_mapsto t (i + j) dq v.
     Proof.
       iIntros "% Hview".
-      iDestruct (raw_array_view_to_mapstos_strong with "Hview") as "(%l & %γ & -> & #Hmeta & H◯ & Hmapstos)".
+      iDestruct (raw_array_view_to_mapstos_strong with "Hview") as "(%l & %γ & -> & #Hmeta & Hlb & Hmapstos)".
       iExists l, γ. iFrame "∗#". iSplit; first done.
       iApply (big_sepL_lookup with "Hmapstos"). done.
     Qed.
@@ -270,10 +285,10 @@ Section raw_array_G.
       ([∗ list] j ↦ v ∈ vs, raw_array_mapsto t (i + j) dq v) -∗
       raw_array_view t i dq vs.
     Proof.
-      iIntros "% #Hmeta #H◯ Hmapstos". simplify.
+      iIntros "% #Hmeta #Hlb Hmapstos". simplify.
       iExists l, γ. repeat iSplit; try done.
       iApply (big_sepL_impl with "Hmapstos").
-      iIntros "!> %j %v %Hlookup (%l' & %γ' & % & #Hmeta' & #H◯' & H↦)". simplify.
+      iIntros "!> %j %v %Hlookup (%l' & %γ' & % & #Hmeta' & #Hlb' & H↦)". simplify.
       done.
     Qed.
     Lemma raw_array_mapstos_to_view t i dq vs :
@@ -282,13 +297,13 @@ Section raw_array_G.
       raw_array_view t i dq vs.
     Proof.
       iIntros "%Hvs Hmapstos".
-      iDestruct (big_sepL_lookup_acc with "Hmapstos") as "((%l & %γ & -> & #Hmeta & #H◯ & H↦) & Hmapstos)".
+      iDestruct (big_sepL_lookup_acc with "Hmapstos") as "((%l & %γ & -> & #Hmeta & #Hlb & H↦) & Hmapstos)".
       { destruct (nth_lookup_or_length vs (length vs - 1) #()); naive_solver lia. }
       assert (S (i + (length vs - 1)) = i + length vs) as Heq; first lia.
-      iEval (rewrite Heq) in "H◯".
+      iEval (rewrite Heq) in "Hlb".
       iDestruct ("Hmapstos" with "[H↦]") as "Hmapstos".
       { iExists l, γ. iEval (rewrite Heq). naive_solver. }
-      iApply (raw_array_mapstos_to_view_strong with "Hmeta H◯ Hmapstos"); first done.
+      iApply (raw_array_mapstos_to_view_strong with "Hmeta Hlb Hmapstos"); first done.
     Qed.
 
     #[local] Lemma raw_array_view_map t i {dq1 vs1} dq2 vs2 :
@@ -302,9 +317,9 @@ Section raw_array_G.
       raw_array_view t i dq2 vs2.
     Proof.
       iIntros "%Hvs2 #H Hview".
-      iDestruct (raw_array_view_to_mapstos_strong with "Hview") as "(%l & %γ & % & #Hmeta & #H◯ & Hmapstos)". simplify.
-      rewrite -Hvs2. iApply (raw_array_mapstos_to_view_strong with "Hmeta H◯ [> Hmapstos]"); first done.
-      iClear "Hmeta H◯". iApply big_sepL_bupd.
+      iDestruct (raw_array_view_to_mapstos_strong with "Hview") as "(%l & %γ & % & #Hmeta & #Hlb & Hmapstos)". simplify.
+      rewrite -Hvs2. iApply (raw_array_mapstos_to_view_strong with "Hmeta Hlb [> Hmapstos]"); first done.
+      iClear "Hmeta Hlb". iApply big_sepL_bupd.
       remember (length vs1) as n eqn:Hvs1.
       iRevert "H Hmapstos". iInduction n as [| n] "IH" forall (i vs1 Hvs1 vs2 Hvs2); iIntros "#H Hmapstos".
       - rewrite (nil_length_inv vs2); done.
@@ -317,15 +332,6 @@ Section raw_array_G.
           iIntros "!> %j %Hj Hmapsto /=".
           iSpecialize ("H" $! (S j) with "[] [Hmapsto]"); first auto with lia;
             rewrite Nat.add_succ_r //.
-    Qed.
-
-    Lemma raw_array_view_persist t i dq vs :
-      raw_array_view t i dq vs ==∗
-      raw_array_view t i DfracDiscarded vs.
-    Proof.
-      iIntros "Hview".
-      iApply (raw_array_view_map with "[] Hview"); first done.
-      iIntros "!> %j _ Hmapsto". iApply (raw_array_mapsto_persist with "Hmapsto").
     Qed.
 
     Lemma raw_array_view_valid t sz i dq vs :
@@ -363,31 +369,6 @@ Section raw_array_G.
       iIntros "!> %j %v1 %v2 % % (Hmapsto1 & Hmapsto2)".
       iApply (raw_array_mapsto_valid_2 with "Hmapsto1 Hmapsto2").
     Qed.
-    Lemma raw_array_view_agree t i dq1 vs1 dq2 vs2 :
-      length vs1 = length vs2 →
-      raw_array_view t i dq1 vs1 -∗
-      raw_array_view t i dq2 vs2 -∗
-      ⌜vs1 = vs2⌝.
-    Proof.
-      iIntros "% Hview1 Hview2".
-      destruct vs1 as [| v1 vs1], vs2 as [| v2 vs2]; try done.
-      iDestruct (raw_array_view_valid_2 with "Hview1 Hview2") as %(_ & ->); try done.
-      list_simplifier. lia.
-    Qed.
-
-    Lemma raw_array_view_exclusive t i vs1 vs2 :
-      0 < length vs1 ≤ length vs2 →
-      raw_array_view t i (DfracOwn 1) vs1 -∗
-      raw_array_view t i (DfracOwn 1) vs2 -∗
-      False.
-    Proof.
-      iIntros "% Hview1 Hview2".
-      destruct vs1 as [| v1 vs1], vs2 as [| v2 vs2]; try naive_solver lia.
-      iDestruct (raw_array_view_to_mapstos with "Hview1") as "(Hmapsto1 & _)".
-      iDestruct (raw_array_view_to_mapstos with "Hview2") as "(Hmapsto2 & _)".
-      iApply (raw_array_mapsto_exclusive with "Hmapsto1 Hmapsto2").
-    Qed.
-
     Lemma raw_array_view_combine t i dq1 vs1 dq2 vs2 :
       length vs1 = length vs2 →
       raw_array_view t i dq1 vs1 -∗
@@ -401,13 +382,64 @@ Section raw_array_G.
         auto.
       }
       iDestruct (raw_array_view_valid_2 with "Hview1 Hview2") as %(_ & <-); [done.. |].
-      iDestruct "Hview1" as "(%l & %γ & % & #Hmeta & #H◯1 & H↦1)".
+      iDestruct "Hview1" as "(%l & %γ & % & #Hmeta & #Hlb1 & H↦1)".
       iDestruct "Hview2" as "(%_l & %_γ & -> & _ & _ & H↦2)". simplify.
       iExists l, γ. iFrame "#". iSplit; first done.
       iDestruct (big_sepL_sep_2 with "H↦1 H↦2") as "H↦".
       iApply (big_sepL_impl with "H↦").
       iIntros "!> %j %v % (H↦1 & H↦2)".
       iDestruct (mapsto_combine with "H↦1 H↦2") as "($ & _)".
+    Qed.
+    Lemma raw_array_view_agree t i dq1 vs1 dq2 vs2 :
+      length vs1 = length vs2 →
+      raw_array_view t i dq1 vs1 -∗
+      raw_array_view t i dq2 vs2 -∗
+      ⌜vs1 = vs2⌝.
+    Proof.
+      iIntros "% Hview1 Hview2".
+      destruct vs1 as [| v1 vs1], vs2 as [| v2 vs2]; try done.
+      iDestruct (raw_array_view_valid_2 with "Hview1 Hview2") as %(_ & ->); try done.
+      list_simplifier. lia.
+    Qed.
+    Lemma raw_array_view_dfrac_ne i t1 dq1 vs1 t2 dq2 vs2 :
+      0 < length vs1 →
+      length vs1 = length vs2 →
+      ¬ ✓ (dq1 ⋅ dq2) →
+      raw_array_view t1 i dq1 vs1 -∗
+      raw_array_view t2 i dq2 vs2 -∗
+      ⌜t1 ≠ t2⌝.
+    Proof.
+      iIntros "% % % Hview1 Hview2" (->).
+      iDestruct (raw_array_view_valid_2 with "Hview1 Hview2") as %?; naive_solver.
+    Qed.
+    Lemma raw_array_view_ne i t1 vs1 t2 dq2 vs2 :
+      0 < length vs1 →
+      length vs1 = length vs2 →
+      raw_array_view t1 i (DfracOwn 1) vs1 -∗
+      raw_array_view t2 i dq2 vs2 -∗
+      ⌜t1 ≠ t2⌝.
+    Proof.
+      intros. iApply raw_array_view_dfrac_ne; [done.. | intros []%(exclusive_l _)].
+    Qed.
+    Lemma raw_array_view_exclusive t i vs1 vs2 :
+      0 < length vs1 ≤ length vs2 →
+      raw_array_view t i (DfracOwn 1) vs1 -∗
+      raw_array_view t i (DfracOwn 1) vs2 -∗
+      False.
+    Proof.
+      iIntros "% Hview1 Hview2".
+      destruct vs1 as [| v1 vs1], vs2 as [| v2 vs2]; try naive_solver lia.
+      iDestruct (raw_array_view_to_mapstos with "Hview1") as "(Hmapsto1 & _)".
+      iDestruct (raw_array_view_to_mapstos with "Hview2") as "(Hmapsto2 & _)".
+      iApply (raw_array_mapsto_exclusive with "Hmapsto1 Hmapsto2").
+    Qed.
+    Lemma raw_array_view_persist t i dq vs :
+      raw_array_view t i dq vs ==∗
+      raw_array_view t i DfracDiscarded vs.
+    Proof.
+      iIntros "Hview".
+      iApply (raw_array_view_map with "[] Hview"); first done.
+      iIntros "!> %j _ Hmapsto". iApply (raw_array_mapsto_persist with "Hmapsto").
     Qed.
 
     Lemma raw_array_view_app t i dq n1 vs1 vs2 :
@@ -416,7 +448,7 @@ Section raw_array_G.
       raw_array_view t (i + n1) dq vs2 -∗
       raw_array_view t i dq (vs1 ++ vs2).
     Proof.
-      iIntros "% (%l & %γ & % & #Hmeta & _ & H↦1) (%_l & %_γ & -> & #_Hmeta & #H◯ & H↦2)". simplify.
+      iIntros "% (%l & %γ & % & #Hmeta & _ & H↦1) (%_l & %_γ & -> & #_Hmeta & #Hlb & H↦2)". simplify.
       iDestruct (meta_agree with "Hmeta _Hmeta") as %<-. iClear "_Hmeta".
       iDestruct (big_sepL_app _ vs1 vs2 with "[$H↦1 H↦2]") as "H↦".
       { iEval (setoid_rewrite (assoc Nat.add)). done. }
@@ -430,10 +462,10 @@ Section raw_array_G.
         raw_array_view t i dq vs1 ∗
         raw_array_view t (i + length vs1) dq vs2.
     Proof.
-      iIntros (->) "(%l & %γ & -> & #Hmeta & #H◯ & H↦)".
+      iIntros (->) "(%l & %γ & -> & #Hmeta & #Hlb & H↦)".
       iDestruct (bi.equiv_entails_1_1 _ _ (big_sepL_app _ vs1 vs2) with "H↦") as "(H↦1 & H↦2)".
       iSplitL "H↦1"; iExists l, γ; iFrame "∗#"; (iSplit; first done).
-      - iApply (raw_array_token_lb_le with "H◯"). rewrite app_length. lia.
+      - iApply (raw_array_token_lb_le with "Hlb"). rewrite app_length. lia.
       - rewrite app_length assoc. setoid_rewrite (assoc Nat.add). auto.
     Qed.
   End raw_array_view.
@@ -464,20 +496,13 @@ Section raw_array_G.
       apply _.
     Qed.
 
-    Lemma raw_array_model_persist t dq vs :
-      raw_array_model t dq vs ==∗
-      raw_array_model t DfracDiscarded vs.
-    Proof.
-      iApply raw_array_view_persist.
-    Qed.
-
     Lemma raw_array_model_valid t sz dq vs :
       0 < length vs →
       raw_array_inv t sz -∗
       raw_array_model t dq vs -∗
       ⌜✓ dq ∧ length vs ≤ sz⌝.
     Proof.
-      intros. iApply raw_array_view_valid. done.
+      apply raw_array_view_valid.
     Qed.
     Lemma raw_array_model_valid_2 t dq1 vs1 dq2 vs2 :
       0 < length vs1 →
@@ -486,7 +511,15 @@ Section raw_array_G.
       raw_array_model t dq2 vs2 -∗
       ⌜✓ (dq1 ⋅ dq2) ∧ vs1 = vs2⌝.
     Proof.
-      intros. iApply raw_array_view_valid_2; done.
+      apply raw_array_view_valid_2.
+    Qed.
+    Lemma raw_array_model_combine t dq1 vs1 dq2 vs2 :
+      length vs1 = length vs2 →
+      raw_array_model t dq1 vs1 -∗
+      raw_array_model t dq2 vs2 -∗
+      raw_array_model t (dq1 ⋅ dq2) vs1.
+    Proof.
+      apply raw_array_view_combine.
     Qed.
     Lemma raw_array_model_agree t dq1 vs1 dq2 vs2 :
       length vs1 = length vs2 →
@@ -494,25 +527,40 @@ Section raw_array_G.
       raw_array_model t dq2 vs2 -∗
       ⌜vs1 = vs2⌝.
     Proof.
-      intros. iApply raw_array_view_agree; done.
+      apply raw_array_view_agree.
     Qed.
-
+    Lemma raw_array_model_dfrac_ne t1 dq1 vs1 t2 dq2 vs2 :
+      0 < length vs1 →
+      length vs1 = length vs2 →
+      ¬ ✓ (dq1 ⋅ dq2) →
+      raw_array_model t1 dq1 vs1 -∗
+      raw_array_model t2 dq2 vs2 -∗
+      ⌜t1 ≠ t2⌝.
+    Proof.
+      apply raw_array_view_dfrac_ne.
+    Qed.
+    Lemma raw_array_model_ne t1 vs1 t2 dq2 vs2 :
+      0 < length vs1 →
+      length vs1 = length vs2 →
+      raw_array_model t1 (DfracOwn 1) vs1 -∗
+      raw_array_model t2 dq2 vs2 -∗
+      ⌜t1 ≠ t2⌝.
+    Proof.
+      apply raw_array_view_ne.
+    Qed.
     Lemma raw_array_model_exclusive t vs1 vs2 :
       0 < length vs1 ≤ length vs2 →
       raw_array_model t (DfracOwn 1) vs1 -∗
       raw_array_model t (DfracOwn 1) vs2 -∗
       False.
     Proof.
-      intros. iApply raw_array_view_exclusive; done.
+      apply raw_array_view_exclusive.
     Qed.
-
-    Lemma raw_array_model_combine t dq1 vs1 dq2 vs2 :
-      length vs1 = length vs2 →
-      raw_array_model t dq1 vs1 -∗
-      raw_array_model t dq2 vs2 -∗
-      raw_array_model t (dq1 ⋅ dq2) vs1.
+    Lemma raw_array_model_persist t dq vs :
+      raw_array_model t dq vs ==∗
+      raw_array_model t DfracDiscarded vs.
     Proof.
-      intros. iApply raw_array_view_combine. done.
+      apply raw_array_view_persist.
     Qed.
 
     Lemma raw_array_model_split t dq vs1 vs2 vs :
@@ -521,7 +569,7 @@ Section raw_array_G.
         raw_array_model t dq vs1 ∗
         raw_array_view t (length vs1) dq vs2.
     Proof.
-      intros. iApply raw_array_view_split. done.
+      apply raw_array_view_split.
     Qed.
   End raw_array_model.
 
@@ -580,14 +628,6 @@ Section raw_array_G.
         iApply (raw_array_span_view_2 with "Hview").
     Qed.
 
-    Lemma raw_array_span_persist t i dq n :
-      raw_array_span t i dq n ==∗
-      raw_array_span t i DfracDiscarded n.
-    Proof.
-      iIntros "(%vs & % & Hview)".
-      iExists vs. iSplitR; first done. iApply raw_array_view_persist. done.
-    Qed.
-
     Lemma raw_array_span_valid t sz i dq n :
       0 < n →
       raw_array_inv t sz -∗
@@ -597,18 +637,16 @@ Section raw_array_G.
       iIntros "% #Hinv (%vs & % & Hview)".
       iDestruct (raw_array_view_valid with "Hinv Hview") as %?; naive_solver.
     Qed.
-
-    Lemma raw_array_span_exclusive t i n1 n2 :
-      0 < n1 ≤ n2 →
-      raw_array_span t i (DfracOwn 1) n1 -∗
-      raw_array_span t i (DfracOwn 1) n2 -∗
-      False.
+    Lemma raw_array_span_valid_2 t i n dq1 dq2 :
+      0 < n →
+      raw_array_span t i dq1 n -∗
+      raw_array_span t i dq2 n -∗
+      ⌜✓ (dq1 ⋅ dq2)⌝.
     Proof.
       iIntros "% (%vs1 & % & Hview1) (%vs2 & % & Hview2)".
-      iApply (raw_array_view_exclusive with "Hview1 Hview2"). lia.
+      iDestruct (raw_array_view_valid_2 with "Hview1 Hview2") as "($ & _)"; naive_solver.
     Qed.
-
-    Lemma raw_array_span_combine t i dq1 dq2 n :
+    Lemma raw_array_span_combine t i n dq1 dq2 :
       raw_array_span t i dq1 n -∗
       raw_array_span t i dq2 n -∗
       raw_array_span t i (dq1 ⋅ dq2) n.
@@ -618,8 +656,42 @@ Section raw_array_G.
       iDestruct (raw_array_view_combine with "Hview1 Hview2")as "Hview"; first done.
       iExists vs. naive_solver.
     Qed.
+    Lemma raw_array_span_dfrac_ne i n t1 dq1 t2 dq2 :
+      0 < n →
+      ¬ ✓ (dq1 ⋅ dq2) →
+      raw_array_span t1 i dq1 n -∗
+      raw_array_span t2 i dq2 n -∗
+      ⌜t1 ≠ t2⌝.
+    Proof.
+      iIntros "% % Hspan1 Hspan2" (->).
+      iDestruct (raw_array_span_valid_2 with "Hspan1 Hspan2") as %?; naive_solver.
+    Qed.
+    Lemma raw_array_span_ne i n t1 t2 dq2 :
+      0 < n →
+      raw_array_span t1 i (DfracOwn 1) n -∗
+      raw_array_span t2 i dq2 n -∗
+      ⌜t1 ≠ t2⌝.
+    Proof.
+      intros. iApply raw_array_span_dfrac_ne; [done.. | intros []%(exclusive_l _)].
+    Qed.
+    Lemma raw_array_span_exclusive t i n1 n2 :
+      0 < n1 ≤ n2 →
+      raw_array_span t i (DfracOwn 1) n1 -∗
+      raw_array_span t i (DfracOwn 1) n2 -∗
+      False.
+    Proof.
+      iIntros "% (%vs1 & % & Hview1) (%vs2 & % & Hview2)".
+      iApply (raw_array_view_exclusive with "Hview1 Hview2"). lia.
+    Qed.
+    Lemma raw_array_span_persist t i dq n :
+      raw_array_span t i dq n ==∗
+      raw_array_span t i DfracDiscarded n.
+    Proof.
+      iIntros "(%vs & % & Hview)".
+      iExists vs. iSplitR; first done. iApply raw_array_view_persist. done.
+    Qed.
 
-    Lemma raw_array_span_append t i dq n1 n2 :
+    Lemma raw_array_span_app t i dq n1 n2 :
       raw_array_span t i dq n1 -∗
       raw_array_span t (i + n1) dq n2 -∗
       raw_array_span t i dq (n1 + n2).
@@ -629,7 +701,7 @@ Section raw_array_G.
       iExists (vs1 ++ vs2). iSplit; first solve_length. done.
     Qed.
 
-    Lemma raw_array_span_split t i dq n1 n2 n :
+    Lemma raw_array_span_split t i dq n n1 n2 :
       n = n1 + n2 →
       raw_array_span t i dq n -∗
         raw_array_span t i dq n1 ∗
@@ -665,9 +737,9 @@ Section raw_array_G.
     { apply lookup_seq. naive_solver lia. }
     iEval (rewrite loc_add_0) in "Hmeta".
     iApply "HΦ".
-    iMod (auth_nat_max_alloc (Z.to_nat sz)) as "(%γ & H●)".
-    iDestruct (auth_nat_max_lb_get with "H●") as "#H◯".
-    iMod (auth_nat_max_auth_persist with "H●") as "#H●".
+    iMod (auth_nat_max_alloc (Z.to_nat sz)) as "(%γ & Hauth)".
+    iDestruct (auth_nat_max_lb_get with "Hauth") as "#Hlb".
+    iMod (auth_nat_max_auth_persist with "Hauth") as "#Hauth".
     iMod (meta_set _ _ γ with "Hmeta") as "#Hmeta"; first done.
     iSplitR; iExists l, γ; iFrame "∗#"; first auto with lia.
     iSplitR; first done.
@@ -676,43 +748,43 @@ Section raw_array_G.
     rewrite Nat.add_0_l //.
   Qed.
 
-  Lemma raw_array_get_spec t sz (i : Z) dq :
+  Lemma raw_array_get_spec t sz (i : Z) dq v E :
     (0 ≤ i < sz)%Z →
-    <<< raw_array_inv t sz | ∀∀ v, raw_array_mapsto t (Z.to_nat i) dq v >>>
-      raw_array_get t #i
-    <<< raw_array_mapsto t (Z.to_nat i) dq v | RET v; True >>>.
+    raw_array_inv t sz -∗
+    raw_array_mapsto t (Z.to_nat i) dq v -∗
+    WP raw_array_get t #i @ E {{ res,
+      ⌜res = v⌝ ∗
+      raw_array_mapsto t (Z.to_nat i) dq v
+    }}.
   Proof.
-    iIntros "% !> %Φ (%l & %γ & -> & #Hmeta & % & #H●) HΦ".
-    wp_rec. wp_pures.
-    iMod "HΦ" as "(%v & (%_l & %_γ & %Heq & #_Hmeta & #H◯ & H↦) & _ & HΦ)". injection Heq as <-.
+    iIntros "% (%l & %γ & -> & #Hmeta & % & #Hauth) (%_l & %_γ & %Heq & #_Hmeta & #Hlb & H↦)". injection Heq as <-.
     iDestruct (meta_agree with "Hmeta _Hmeta") as %<-. iClear "_Hmeta".
+    wp_rec. wp_pures.
     rewrite Z2Nat.id; last lia. wp_load.
-    iApply ("HΦ" with "[H↦] [//]").
-    iExists l, γ. iFrame "∗#". iSplit; first done.
-    rewrite Z2Nat.id //. lia.
+    iSplitR; first done. iExists l, γ. rewrite Z2Nat.id //; last lia. naive_solver.
   Qed.
 
-  Lemma raw_array_set_spec t sz i v :
+  Lemma raw_array_set_spec t sz i w v E :
     (0 ≤ i < sz)%Z →
-    <<< raw_array_inv t sz | ∀∀ w, raw_array_mapsto t (Z.to_nat i) (DfracOwn 1) w >>>
-      raw_array_set t #i v
-    <<< raw_array_mapsto t (Z.to_nat i) (DfracOwn 1) v | RET #(); True >>>.
+    raw_array_inv t sz -∗
+    raw_array_mapsto t (Z.to_nat i) (DfracOwn 1) w -∗
+    WP raw_array_set t #i v @ E {{ res,
+      ⌜res = #()⌝ ∗
+      raw_array_mapsto t (Z.to_nat i) (DfracOwn 1) v
+    }}.
   Proof.
-    iIntros "% !> %Φ (%l & %γ & -> & #Hmeta & % & #H●) HΦ".
-    wp_rec. wp_pures.
-    iMod "HΦ" as "(%w & (%_l & %_γ & %Heq & #_Hmeta & #H◯ & H↦) & _ & HΦ)". injection Heq as <-.
+    iIntros "% (%l & %γ & -> & #Hmeta & % & #Hauth) (%_l & %_γ & %Heq & #_Hmeta & #Hlb & H↦)". injection Heq as <-.
     iDestruct (meta_agree with "Hmeta _Hmeta") as %<-. iClear "_Hmeta".
+    wp_rec. wp_pures.
     rewrite Z2Nat.id; last lia. wp_store.
-    iApply ("HΦ" with "[H↦] [//]").
-    iExists l, γ. iFrame "∗#". iSplit; first done.
-    rewrite Z2Nat.id //. lia.
+    iSplitR; first done. iExists l, γ. rewrite Z2Nat.id; last lia. naive_solver.
   Qed.
 
   Lemma raw_array_unboxed t sz :
     raw_array_inv t sz -∗
     ⌜val_is_unboxed t⌝.
   Proof.
-    iIntros "(%l & %γ & -> & #Hmeta & % & #H●) //".
+    iIntros "(%l & %γ & -> & #Hmeta & % & #Hauth) //".
   Qed.
 End raw_array_G.
 
